src/Step.hs
@@ -18,22 +18,14 @@ lam lambda =
   case lambda of {
    Build_Lambda _ lam0 -> lam0}
 
-data Term v =
-   Var v
- | Pass (Term v) (Term v)
- | Lam_ (v -> Term v)
+data Ast v =
+   Ast_var v
+ | Ast_app (Ast v) (Ast v)
+ | Ast_lam (v -> Ast v)
 
-term_lambda :: Lambda (Term a1)
-term_lambda =
-  Build_Lambda (\x x0 -> Pass x x0) (\f -> Lam_ (\x -> f (Var x)))
-
-type Store v = v -> Term v
-
-put :: (EqDec a1) -> (a1 -> Term a1) -> a1 -> (Term a1) -> Store a1
-put h old x e x' =
-  case eq_decide h x x' of {
-   Prelude.True -> e;
-   Prelude.False -> old x'}
+ast_lambda :: Lambda (Ast a1)
+ast_lambda =
+  Build_Lambda (\x x0 -> Ast_app x x0) (\f -> Ast_lam (\x -> f (Ast_var x)))
 
 data Font v =
    Build_font v (Font v) (Font v)
@@ -45,30 +37,36 @@ head f =
 
 data Stack v =
    Hole
- | Lpass (Stack v) (Term v)
+ | Lpass (Stack v) (Ast v)
 
-type Heap v = [] ((,) v (Term v))
+type Heap v = [] ((,) v (Ast v))
 
-arbitrary :: Term a1
+arbitrary :: Ast a1
 arbitrary =
-  lam term_lambda (\x -> x)
+  lam ast_lambda (\x -> x)
 
-lookup :: (EqDec a1) -> (Heap a1) -> Store a1
+lookup :: (EqDec a1) -> (Heap a1) -> a1 -> Ast a1
 lookup h hp =
   case hp of {
    [] -> (\_ -> arbitrary);
-   (:) p t -> case p of {
-               (,) x' h0 -> put h (lookup h t) x' h0}}
+   (:) p t ->
+    case p of {
+     (,) x' h0 ->
+      let {t' = lookup h t} in
+      (\x ->
+      case eq_decide h x x' of {
+       Prelude.True -> h0;
+       Prelude.False -> t' x})}}
 
-type State v = (,) ((,) (Heap v) (Stack v)) (Term v)
+type State v = (,) ((,) (Heap v) (Stack v)) (Ast v)
 
-go :: (EqDec a1) -> (Font a1) -> (Heap a1) -> (Stack a1) -> (Term a1) ->
+go :: (EqDec a1) -> (Font a1) -> (Heap a1) -> (Stack a1) -> (Ast a1) ->
       Prelude.Maybe (State a1)
 go h fnt s k e =
   case e of {
-   Var x -> Prelude.Just ((,) ((,) s k) (lookup h s x));
-   Pass e0 e1 -> Prelude.Just ((,) ((,) s (Lpass k e1)) e0);
-   Lam_ f ->
+   Ast_var x -> Prelude.Just ((,) ((,) s k) (lookup h s x));
+   Ast_app e0 e1 -> Prelude.Just ((,) ((,) s (Lpass k e1)) e0);
+   Ast_lam f ->
     case k of {
      Hole -> Prelude.Nothing;
      Lpass k' e0 ->
